Introduce [Vale.Transformers.Common] to make the dep mgmt easier

vale/code/lib/transformers/Vale.Transformers.Transform.fsti
@@ -23,18 +23,10 @@ module Vale.Transformers.Transform
 open Vale.X64.Machine_s
 open Vale.Def.PossiblyMonad
 open Vale.X64.Decls
+open Vale.Transformers.Common
 
-/// Common definitions amongst transformations.
-
-let equiv_states (s1 s2:va_state) =
-  let open Vale.X64.State in
-  s1.vs_ok == s2.vs_ok /\
-  Vale.X64.Regs.equal s1.vs_regs s2.vs_regs /\
-  Vale.X64.Flags.sel fCarry s1.vs_flags == Vale.X64.Flags.sel fCarry s2.vs_flags /\
-  Vale.X64.Flags.sel fOverflow s1.vs_flags == Vale.X64.Flags.sel fOverflow s2.vs_flags /\
-  s1.vs_heap == s2.vs_heap /\
-  s1.vs_stack == s2.vs_stack /\
-  s1.vs_stackTaint == s2.vs_stackTaint
+(* Re-expose [equiv_states], so that Common doesn't need to be imported *)
+unfold let equiv_states (s1 s2:va_state) = equiv_states s1 s2
 
 /// The Instruction Reordering Transformation
 
